src/Pipit.Sugar.Check.fst
@@ -27,19 +27,22 @@ let contract_system_induct_k1' (#t: table) (#c: context t) (#a: t.ty) (r: XCC.ce
   SI.induct1 (SX.system_of_contract r g i)
 
 let stream_of_contract1 (#t: table) (#a #b: t.ty) (#r: XCC.cexp t [a] t.propty) (#g: XCC.cexp t [b; a] t.propty) (contr: contract t [a] b r g): stream t a -> stream t b =
-  // let rely = XC.bless r in
+  // let rely = XCC.bless r in
   let rely = r in
-  let guar = XC.bless g in
-  let impl = XC.bless contr in
+  let guar = XCC.bless g in
+  let impl = XCC.bless contr in
   let e = XContract PM.PSUnknown rely guar impl in
+  // TODO:ADMIT: bless is sealed
+  assume (XC.sealed false impl);
+  assume (XC.sealed false guar);
   // TODO:ADMIT: requires contract_check
   assume (XC.contract_valid r g contr ==> XC.check_all PM.check_mode_valid e);
   stream_of_exp1 e
 
 // let stream_of_contract2 (#t: table) (#a #b #c: t.ty) (contr: _contract t [a; b] c { XC.contract_valid contr.rely contr.guar contr.impl }): stream t a -> stream t b -> stream t c =
-//   let rely = XC.bless contr.rely in
-//   let guar = XC.bless contr.guar in
-//   let impl = XC.bless contr.impl in
+//   let rely = XCC.bless contr.rely in
+//   let guar = XCC.bless contr.guar in
+//   let impl = XCC.bless contr.impl in
 //   let e = XContract PM.PSUnknown rely guar impl in
 //   // TODO:ADMIT: requires contract_check
 //   assume (XC.check_all PM.check_mode_valid e);
@@ -53,19 +56,19 @@ let exp_of_stream3 (#t: table) (#a #b #c #d: t.ty) (f: stream t a -> stream t b 
 
 
 let stream_of_checked0 (#t: table) (#a: t.ty) (e: XCC.cexp t [] a { XC.check_all PM.check_mode_unknown e }): stream t a =
-  let e' = XC.bless e in
+  let e' = XCC.bless e in
   stream_of_exp0 e'
 
 let stream_of_checked1 (#t: table) (#a #b: t.ty) (e: XCC.cexp t [a] b { XC.check_all PM.check_mode_unknown e }): stream t a -> stream t b =
-  let e' = XC.bless e in
+  let e' = XCC.bless e in
   stream_of_exp1 e'
 
 let stream_of_checked2 (#t: table) (#a #b #c: t.ty) (e: XCC.cexp t [a; b] c { XC.check_all PM.check_mode_unknown e }): stream t a -> stream t b -> stream t c =
-  let e' = XC.bless e in
+  let e' = XCC.bless e in
   stream_of_exp2 e'
 
 let stream_of_checked3 (#t: table) (#a #b #c #d: t.ty) (e: XCC.cexp t [a; b; c] d { XC.check_all PM.check_mode_unknown e }): stream t a -> stream t b -> stream t c -> stream t d =
-  let e' = XC.bless e in
+  let e' = XCC.bless e in
   stream_of_exp3 e'
 
 
